cfrontend/BeePL_proof.v
@@ -131,45 +131,76 @@ Admitted.
 
 Section specifications.
 
-(* Complete me *)
-Inductive tr_expr_expr : vmap -> BeePL.expr -> Csyntax.expr -> Prop :=
-| tr_val_unit : forall le cv ct, (* Fix me *)
-                transBeePL_value_cvalue Vunit = cv ->
-                transBeePL_type (Ptype Tunit) = OK ct ->
-                tr_expr_expr le (BeePL.Val Vunit (Ptype Tunit)) (Csyntax.Eval cv ct)
-| tr_val_int : forall le i sz s a,
-               tr_expr_expr le (BeePL.Val (Vint i) (Ptype (Tint sz s a))) 
-                               (Csyntax.Eval (Values.Vint i) (Ctypes.Tint sz s a))
-| tr_val_long : forall le i s a,
-                tr_expr_expr le (BeePL.Val (Vint64 i) (Ptype (Tlong s a))) 
-                                (Csyntax.Eval (Values.Vlong i) (Ctypes.Tlong s a))
-| tr_val_loc : forall le l ofs t ct,
+(* Simpler specification for expressions translations *) 
+Inductive tr_expr_expr : BeePL.expr -> Csyntax.expr -> Prop :=
+| tr_val_unit : forall t ct, (* Fix me *)
+                transBeePL_type t = OK ct ->
+                tr_expr_expr (BeePL.Val Vunit t) (Csyntax.Eval (transBeePL_value_cvalue Vunit) ct)
+| tr_val_int : forall i t ct,
                transBeePL_type t = OK ct ->
-               tr_expr_expr le (BeePL.Val (Vloc l ofs) t) (Csyntax.Eval (Values.Vptr l ofs) ct)
-| tr_var : forall (le:BeePL.vmap) (le':Csem.env) x ct l,
+               tr_expr_expr (BeePL.Val (Vint i) t) (Csyntax.Eval (Values.Vint i) ct)
+| tr_val_long : forall i t ct,
+                tr_expr_expr (BeePL.Val (Vint64 i) t) (Csyntax.Eval (Values.Vlong i) ct)
+| tr_val_loc : forall l ofs t ct,
+               transBeePL_type t = OK ct ->
+               tr_expr_expr (BeePL.Val (Vloc l ofs) t) (Csyntax.Eval (Values.Vptr l ofs) ct)
+| tr_var : forall x ct,
            transBeePL_type x.(vtype) = OK ct ->
-           le ! (vname x) = Some (l, x.(vtype)) ->
-           le' ! (vname x) = Some (l, ct) ->
-           tr_expr_expr le (BeePL.Var x) (Csyntax.Evar x.(vname) ct)
-| tr_const_int : forall le i t ct,
+           tr_expr_expr (BeePL.Var x) (Csyntax.Evar x.(vname) ct)
+| tr_const_int : forall i t ct ,
                  transBeePL_type t = OK ct ->
-                 tr_expr_expr le (BeePL.Const (ConsInt i) t) (Csyntax.Eval (Values.Vint i) ct)
-| tr_const_long : forall le i t ct,
+                 tr_expr_expr (BeePL.Const (ConsInt i) t) (Csyntax.Eval (Values.Vint i) ct)
+| tr_const_long : forall i t ct,
                   transBeePL_type t = OK ct ->
-                  tr_expr_expr le (BeePL.Const (ConsLong i) t) (Csyntax.Eval (Values.Vlong i) ct)
-| tr_const_unit : forall le cv ct, (* Fix me *)
+                  tr_expr_expr (BeePL.Const (ConsLong i) t) (Csyntax.Eval (Values.Vlong i) ct)
+| tr_const_unit : forall cv ct, (* Fix me *)
                   transBeePL_value_cvalue Vunit = cv ->
                   transBeePL_type (Ptype Tunit) = OK ct ->
-                  tr_expr_expr le (BeePL.Const ConsUnit (Ptype Tunit)) (Csyntax.Eval cv ct)
-| tr_prim_op : forall le o e1 t ct ce1, 
-               transBeePL_type t = OK ct ->
-               tr_expr_expr le e1 ce1 ->
-               tr_expr_expr le (BeePL.Prim (Uop o) (e1 :: nil) t) (Csyntax.Eunop o ce1 ct)
-| tr_prim_bop : forall le o e1 e2 t ct ce1 ce2,
+                  tr_expr_expr (BeePL.Const ConsUnit (Ptype Tunit)) (Csyntax.Eval cv ct)
+| tr_prim_ref : forall e t ct ce, 
                 transBeePL_type t = OK ct ->
-                tr_expr_expr le e1 ce1 ->
-                tr_expr_expr le e2 ce2 ->
-                tr_expr_expr le (BeePL.Prim (Bop o) (e1 :: e2 :: nil) t) (Csyntax.Ebinop o ce1 ce2 ct).
+                tr_expr_expr e ce ->
+                tr_expr_expr (BeePL.Prim Ref (e :: nil) t) (Csyntax.Eaddrof ce ct)
+| tr_prim_deref : forall e t ct ce,
+                  transBeePL_type t = OK ct ->
+                  tr_expr_expr e ce ->
+                  tr_expr_expr (BeePL.Prim Deref (e :: nil) t) (Csyntax.Ederef ce ct)
+| tr_prim_massgn : forall e1 e2 t ce1 ce2 ct,
+                   transBeePL_type t = OK ct ->
+                   tr_expr_expr e1 ce1 ->
+                   tr_expr_expr e2 ce2 ->
+                   tr_expr_expr (BeePL.Prim Massgn (e1 :: e2 :: nil) t) (Csyntax.Eassign ce1 ce2 ct)
+| tr_prim_op : forall o e1 t ct ce1, 
+               transBeePL_type t = OK ct ->
+               tr_expr_expr e1 ce1 ->
+               tr_expr_expr (BeePL.Prim (Uop o) (e1 :: nil) t) (Csyntax.Eunop o ce1 ct)
+| tr_prim_bop : forall o e1 e2 t ct ce1 ce2,
+                transBeePL_type t = OK ct ->
+                tr_expr_expr e1 ce1 ->
+                tr_expr_expr e2 ce2 ->
+                tr_expr_expr (BeePL.Prim (Bop o) (e1 :: e2 :: nil) t) (Csyntax.Ebinop o ce1 ce2 ct)
+| tr_prim_run : forall h t,
+                tr_expr_expr (BeePL.Prim (Run h) nil t) (Eval (Values.Vundef) Tvoid) (* Fix me *)
+| tr_bind : forall x t e e' t' ct ct' ce ce', (* Fix me *)
+            transBeePL_type t = OK ct ->
+            transBeePL_type t' = OK ct' ->
+            tr_expr_expr e ce ->
+            tr_expr_expr e' ce' ->
+            tr_expr_expr (BeePL.Bind x t e e' t') (Csyntax.Ecomma (Eassign (Csyntax.Evar x ct) ce ct) ce' ct')
+| tr_cond : forall e1 e2 e3 t ct ce1 ce2 ce3,
+            transBeePL_type t = OK ct ->
+            tr_expr_expr e1 ce1 ->
+            tr_expr_expr e2 ce2 ->
+            tr_expr_expr e3 ce3 ->
+            tr_expr_expr (BeePL.Cond e1 e2 e3 t) (Csyntax.Econdition ce1 ce2 ce3 ct)
+| tr_unit : forall t ct, (* Fix me *)
+            transBeePL_type t = OK ct ->
+            tr_expr_expr (BeePL.Unit t) (Csyntax.Eval (transBeePL_value_cvalue Vunit) ct)
+| tr_addr : forall l ofs ct,
+            transBeePL_type l.(ltype) = OK ct ->
+            tr_expr_expr (BeePL.Addr l ofs) (Csyntax.Eloc l.(lname) ofs l.(lbitfield) ct)
+| tr_hexpr : forall h e t, (* Fix me *)
+             tr_expr_expr (BeePL.Hexpr h e t) (Eval (Values.Vundef) Tvoid). 
 
 (* Complete me *)
 Inductive tr_expr_stmt : BeePL.expr -> Csyntax.statement -> Prop :=
@@ -178,10 +209,23 @@ Inductive tr_expr_stmt : BeePL.expr -> Csyntax.statement -> Prop :=
               transBeePL_value_cvalue v = cv ->
               tr_expr_stmt (BeePL.Val v t) (Csyntax.Sreturn (Some (Eval (transBeePL_value_cvalue v) ct))).
 
-Lemma tranBeePL_expr_expr_spec: forall le e ce,
+Lemma tranBeePL_expr_expr_spec: forall e ce,
 transBeePL_expr_expr e = OK ce ->
-tr_expr_expr le e ce.
+tr_expr_expr e ce.
 Proof.
+move=> e ce ht. elim: e ht=> //=.
+(* val *)
++ move=> v t ht. monadInv ht.
+  case: v=> //=.
+  + by apply tr_val_unit.
+  + move=> i. by apply tr_val_int.
+  + move=> i. by apply tr_val_long.
+  move=> l ofs. by apply tr_val_loc.
+(* var *)
++ move=> vi ht. monadInv ht.
+  by apply tr_var.
+(* const *)
++ move=> [].
 Admitted.
 
 Lemma tranBeePL_expr_stmt_spec: forall e ce,
@@ -281,6 +325,84 @@ Qed.
 
 End specifications.
 
+Section Advanced_specifications.
+
+Inductive sim_bexpr_cexpr : vmap -> BeePL.expr -> Csyntax.expr -> Prop :=
+| sim_val_unit : forall le t ct, (* Fix me *)
+                 transBeePL_type t = OK ct ->
+                 sim_bexpr_cexpr le (BeePL.Val Vunit t) (Csyntax.Eval (transBeePL_value_cvalue Vunit) ct)
+| sim_val_int : forall le i t ct,
+                transBeePL_type t = OK ct ->
+                sim_bexpr_cexpr le (BeePL.Val (Vint i) t) (Csyntax.Eval (Values.Vint i) ct)
+| sim_val_long : forall le i t ct,
+                 sim_bexpr_cexpr le (BeePL.Val (Vint64 i) t) (Csyntax.Eval (Values.Vlong i) ct)
+| sim_val_loc : forall le l ofs t ct,
+                transBeePL_type t = OK ct ->
+                sim_bexpr_cexpr le (BeePL.Val (Vloc l ofs) t) (Csyntax.Eloc l ofs Full ct)
+| sim_var_local : forall (le:BeePL.vmap) (le':Csem.env) x ct,
+                  transBeePL_type x.(vtype) = OK ct ->
+                  (forall le' id, if isSome (le ! id) 
+                                    then (forall l, le ! id = Some (l, vtype x) /\ le' ! id = Some (l, ct)) 
+                                    else le ! id = None /\ le' ! id = None) ->
+                  sim_bexpr_cexpr le (BeePL.Var x) (Csyntax.Evar x.(vname) ct)
+| sim_const_int : forall le i t ct,
+                  transBeePL_type t = OK ct ->
+                  sim_bexpr_cexpr le (BeePL.Const (ConsInt i) t) (Csyntax.Eval (Values.Vint i) ct)
+| sim_const_long : forall le i t ct,
+                   transBeePL_type t = OK ct ->
+                   sim_bexpr_cexpr le (BeePL.Const (ConsLong i) t) (Csyntax.Eval (Values.Vlong i) ct)
+| sim_const_unit : forall le cv ct, (* Fix me *)
+                   transBeePL_value_cvalue Vunit = cv ->
+                   transBeePL_type (Ptype Tunit) = OK ct ->
+                   sim_bexpr_cexpr le (BeePL.Const ConsUnit (Ptype Tunit)) (Csyntax.Eval cv ct)
+| sim_prim_ref : forall le e t ct ce, 
+                 transBeePL_type t = OK ct ->
+                 sim_bexpr_cexpr le e ce ->
+                 sim_bexpr_cexpr le (BeePL.Prim Ref (e :: nil) t) (Csyntax.Eaddrof ce ct)
+| sim_prim_deref : forall le e t ct ce,
+                   transBeePL_type t = OK ct ->
+                   sim_bexpr_cexpr le e ce ->
+                   sim_bexpr_cexpr le (BeePL.Prim Deref (e :: nil) t) (Csyntax.Ederef ce ct)
+| sim_prim_massgn : forall le e1 e2 t ce1 ce2 ct,
+                    transBeePL_type t = OK ct ->
+                    sim_bexpr_cexpr le e1 ce1 ->
+                    sim_bexpr_cexpr le e2 ce2 ->
+                    sim_bexpr_cexpr le (BeePL.Prim Massgn (e1 :: e2 :: nil) t) (Csyntax.Eassign ce1 ce2 ct)
+| sim_prim_op : forall le o e1 t ct ce1, 
+                transBeePL_type t = OK ct ->
+                sim_bexpr_cexpr le e1 ce1 ->
+                sim_bexpr_cexpr le (BeePL.Prim (Uop o) (e1 :: nil) t) (Csyntax.Eunop o ce1 ct)
+| sim_prim_bop : forall le o e1 e2 t ct ce1 ce2,
+                 transBeePL_type t = OK ct ->
+                 sim_bexpr_cexpr le e1 ce1 ->
+                 sim_bexpr_cexpr le e2 ce2 ->
+                 sim_bexpr_cexpr le (BeePL.Prim (Bop o) (e1 :: e2 :: nil) t) (Csyntax.Ebinop o ce1 ce2 ct)
+| sim_prim_run : forall le h t,
+                 sim_bexpr_cexpr le (BeePL.Prim (Run h) nil t) (Eval (Values.Vundef) Tvoid) (* Fix me *)
+| sim_bind : forall le x t e e' t' ct ct' ce ce', (* Fix me *)
+             transBeePL_type t = OK ct ->
+             transBeePL_type t' = OK ct' ->
+             sim_bexpr_cexpr le e ce ->
+             sim_bexpr_cexpr le e' ce' ->
+             sim_bexpr_cexpr le (BeePL.Bind x t e e' t') (Csyntax.Ecomma (Eassign (Csyntax.Evar x ct) ce ct) ce' ct')
+| sim_cond : forall le e1 e2 e3 t ct ce1 ce2 ce3,
+             transBeePL_type t = OK ct ->
+             sim_bexpr_cexpr le e1 ce1 ->
+             sim_bexpr_cexpr le e2 ce2 ->
+             sim_bexpr_cexpr le e3 ce3 ->
+             sim_bexpr_cexpr le (BeePL.Cond e1 e2 e3 t) (Csyntax.Econdition ce1 ce2 ce3 ct)
+| sim_unit : forall le t ct, (* Fix me *)
+             transBeePL_type t = OK ct ->
+             sim_bexpr_cexpr le (BeePL.Unit t) (Csyntax.Eval (transBeePL_value_cvalue Vunit) ct)
+| sim_addr : forall le l ofs ct,
+             transBeePL_type l.(ltype) = OK ct ->
+             sim_bexpr_cexpr le (BeePL.Addr l ofs) (Csyntax.Eloc l.(lname) ofs l.(lbitfield) ct)
+| sim_hexpr : forall le h e t, (* Fix me *)
+              sim_bexpr_cexpr le (BeePL.Hexpr h e t) (Eval (Values.Vundef) Tvoid). 
+
+      
+End Advanced_specifications.
+
 Section semantic_preservation.
 
 Variable bprog : BeePL.program.
@@ -338,15 +460,26 @@ transBeePL_type (BeePL.fn_return f) = OK (Csyntax.fn_return tf).
 Proof.
 Admitted.
 
-
 (* Preservation of deref_addr between BeePL and Csyntax *) 
-Lemma deref_addr_translated : forall ty m addr ofs bf v cty tr cv,
+Lemma deref_addr_translated : forall ty m addr ofs bf v cty cv,
 deref_addr ty m addr ofs bf v ->
 transBeePL_type ty = OK cty ->
 transBeePL_value_cvalue v = cv ->
-Csem.deref_loc cge cty m addr ofs bf tr cv.
+Csem.deref_loc cge cty m addr ofs bf Events.E0 cv.
 Proof.
-Admitted.
+move=> ty m addr ofs bf v cty cv hd ht hv. inversion hd; subst.
++ apply Csem.deref_loc_value with chunk.
+  + by have := BeePL_auxlemmas.access_mode_preserved ty cty (By_value chunk) H ht.
+  + by have := non_volatile_type_preserved ty cty H0 ht.
+  rewrite /transBeePL_value_cvalue in H1. rewrite H1 /=.
+  case: v hd H2=> //=.
+  + by case: v0 H1=> //=.
+  + by case: v0 H1=> //= i H1 i' Hd [] hi; subst.
+  + by case: v0 H1=> //= i H1 i' Hd [] hi; subst.
+  by case: v0 H1=> //= l i H1 l' i' Hd [] h1 h2; subst.
+apply Csem.deref_loc_reference.
+by have := BeePL_auxlemmas.access_mode_preserved ty cty By_reference H ht.
+Qed.
 
 (* Preservation of assign_addr between BeePL and Csyntax *) 
 Lemma assgn_addr_translated : forall ty m addr ofs bf v m' cty tr cv v' cv',
@@ -358,7 +491,113 @@ Csem.assign_loc cge cty m addr ofs bf cv tr m' cv'.
 Proof.
 Admitted.
 
-(* Preservation of expression semantics with respect to small-step semantics *)
+(* Big step semantics with rvalue *) 
+Lemma bsem_cexpr_rval : forall e ce m m' v ct,
+bsem_expr bge benv m e m' v ->
+transBeePL_type (typeof_expr e) = OK ct ->
+transBeePL_expr_expr e = OK ce ->
+exists tr, eval_expr cge cenv m Csem.RV ce tr m' (Eval (transBeePL_value_cvalue v) ct).
+Proof.
+Admitted.
+
+
+(* Big step semantics with rvalue *) 
+Lemma bsem_cexpr_lval : forall e ce m m' v ct l ofs bf,
+bsem_expr bge benv m e m' v ->
+transBeePL_type (typeof_expr e) = OK ct ->
+transBeePL_expr_expr e = OK ce ->
+exists tr, eval_expr cge cenv m Csem.LV ce tr m' (Eloc l ofs bf ct).
+Proof.
+Admitted.
+
+
+(* Big step semantics of BeePL to big step semantics of Cstrategy *) 
+Lemma bsem_cexpr_preserve : forall m e m' v ce,
+bsem_expr bge benv m e m' v ->
+transBeePL_expr_expr e = OK ce ->
+sim_bexpr_cexpr benv e ce ->
+exists cv tr cm', eval_expression cge cenv m ce tr cm' cv /\
+transBeePL_value_cvalue v = cv.
+Proof.
+move=> m e m' v ce. move: m m' v. elim: e=> //=.
+(* Val *)
++ move=> v' t' m m' v he ht hs. monadInv ht; subst; rewrite /=.
+  exists (transBeePL_value_cvalue v'). exists Events.E0. exists m. split=> //=.
+  + apply eval_expression_intro with (Eval (transBeePL_value_cvalue v') x).
+    apply eval_val. by apply esr_val.
+  by inversion he; subst.
+(* Var *)
++ move=> vi m m' v he ht hs. monadInv ht; subst; rewrite /=.
+  inversion he; subst.
+  (* local *)
+  + admit.
+  (* global *)
+  admit.
+(* Const *)
++ admit.
+(* App *)
++ admit.
+(* Builtin *)
++ move=> [].   
+  (* Ref *)
+  + move=> es t m m' v he ht hs. monadInv ht; subst; rewrite /=.
+    case: es he hs EQ=> //=.
+    + move=> he. by inversion he.
+    move=> e es he. inversion he; subst.
+    move=> hs ht. monadInv ht; subst.
+    rewrite /exprlist_list_expr /=. rewrite /exprlist_list_expr /= in hs.
+    have [tr htr] := bsem_cexpr_lval e x1 m m' v0 ct l Ptrofs.zero Full H4 H7 EQ.
+    exists (Values.Vptr l Ptrofs.zero). eexists tr. exists m'. split=> //=.
+    apply eval_expression_intro with (Csyntax.Eaddrof (Eloc l Ptrofs.zero Full ct) x0).
+    + apply eval_addrof. by inversion hs; subst. 
+    apply esr_addrof. by apply esl_loc.
+  (* Deref *)
+  + move=> es t m m' v he ht hs. monadInv ht; subst; rewrite /=.
+    case: es he hs EQ=> //=.
+    + move=> he. by inversion he.
+    move=> e es he. inversion he; subst.
+    move=> hs ht. monadInv ht; subst.
+    rewrite /exprlist_list_expr /=. rewrite /exprlist_list_expr /= in hs.
+    inversion hs; subst; rewrite /=.
+    admit.
+  (* Massgn *)
+  + admit.
+  (* Op *)
+  + move=> u es t m m' v he ht hs. monadInv ht; subst; rewrite /=.
+    inversion hs; subst. inversion he; subst. 
+    rewrite /exprlist_list_expr /= in EQ. monadInv EQ; subst; rewrite /=. 
+    have [tr h] := bsem_cexpr_rval e1 x1 m m' v0 ct H3 H7 EQ0.
+    exists v'. exists tr. exists m'. split=> //=. 
+    + apply eval_expression_intro with (Csyntax.Eunop u (Eval (transBeePL_value_cvalue v0) ct) x0). 
+      + by apply eval_unop. 
+      apply esr_unop with (transBeePL_value_cvalue v0).
+      + by apply esr_val.
+      by have heq := typec_expr e1 ct x1 H7 EQ0; subst.
+    by have := bv_cv_reflex v' v H11.
+  (* Bop *)
+  + move=> b es t m m' v he ht hs. monadInv ht; subst; rewrite /=.
+    case: es he hs EQ=> //=.
+    + move=> he. by inversion he.
+    move=> e es he. inversion he; subst.
+    move=> hs ht. monadInv ht; subst. inversion EQ2. monadInv EQ2; subst; rewrite /=.
+    rewrite /exprlist_list_expr /=. rewrite /exprlist_list_expr /= in hs.
+    inversion hs; subst; rewrite /=.
+    have [tr1 htr1] := bsem_cexpr_rval e x1 m hm' v1 ct1 H3 H7 EQ.
+    have [tr2 htr2] := bsem_cexpr_rval e2 x hm' m' v2 ct2 H4 H10 EQ0.
+    exists v0. exists (Events.Eapp tr1 tr2). exists m'. split=> //=.
+    + apply eval_expression_intro with 
+      (Csyntax.Ebinop b (Eval (transBeePL_value_cvalue v1) ct1) 
+                        (Eval (transBeePL_value_cvalue v2) ct2) x0).
+      + apply eval_binop with hm'.
+        + by apply htr1.
+        by apply htr2.
+      apply esr_binop with (transBeePL_value_cvalue v1) (transBeePL_value_cvalue v2).
+      + by apply esr_val.
+      by apply esr_val.    
+Admitted.
+
+
+(* Returns true if the expression can be in the position of LV *)
 Definition is_lbeepl (e : BeePL.expr) : bool :=
 match e with 
 | Val v t => false
@@ -376,18 +615,116 @@ match e with
 | Bind x t e e' t' => false
 | Cond e1 e2 e3 t => false
 | Unit t => false
+| Addr l ofs => false 
+| Hexpr m e t => false (* Fix me *)
+end.
+
+Section Is_simples.
+
+Variable is_simple : BeePL.expr -> bool.
+
+Fixpoint is_simples (es : list BeePL.expr) : bool :=
+match es with 
+| nil => true 
+| e :: es => is_simple e && is_simples es
+end.
+
+End Is_simples.
+
+(* Return true for simple (non-effectful) expressions *)
+Fixpoint is_simple (e : BeePL.expr) : bool :=
+match e with 
+| Val v t => true
+| Var v => true 
+| Const c t => true
+| App id e es t => false 
+| Prim b es t => match b with 
+                 | Ref => is_simples is_simple es
+                 | Deref => is_simples is_simple es 
+                 | Massgn => is_simples is_simple es 
+                 | Uop o => is_simples is_simple es
+                 | Bop o => is_simples is_simple es
+                 | Run h => false (* Fix me *)
+                 end
+| Bind x t e e' t' => false
+| Cond e1 e2 e3 t => false
+| Unit t => true
 | Addr l ofs => true 
 | Hexpr m e t => false (* Fix me *)
 end.
 
+Lemma bsem_lexpr_preserve : forall m e m' v ce,
+bsem_expr bge benv m e m' v ->
+is_lbeepl e = true ->
+transBeePL_expr_expr e = OK ce ->
+sim_bexpr_cexpr benv e ce ->
+exists l ofs bv, eval_simple_lvalue cge cenv m ce l ofs bv. 
+Proof.
+move=> m e m' v ce he hl ht htr. elim: e he hl ht htr=> //=.
+(* Var *)
++ move=> vi he _ ht htr. inversion he; subst.
+  (* local *)
+  + monadInv ht; subst. inversion htr; subst.
+    move: (H5 cenv (vname vi)). case: ifP=> //= h h'.
+    exists l, Ptrofs.zero, Full. apply esl_var_local.
+    move: (h' l). by move=> [] h1 h2.
+  + case: h'=> //= h1 h2. by rewrite H0 in h1.
+  (* global *)
+  monadInv ht; subst. inversion htr; subst.
+  move: (H6 cenv (vname vi)). case: ifP=> //= h h'.
+  + by rewrite H0 in h.
+  case: h'=> [] h1 h2.
+  exists l, Ptrofs.zero, Full. apply esl_var_global.
+  + by apply h2.
+  by rewrite symbols_preserved.
+(* Builtin-deref *)
++ move=> [] //= es t he _ ht htr. monadInv ht.
+  inversion htr; subst. rewrite /transBeePL_expr_exprs /= in EQ. 
+  monadInv EQ; subst. rewrite /exprlist_list_expr /=. 
+  inversion he; subst. exists l, ofs, Full.
+  (*by have := eval_Ederef m e m' l ofs x1 x0 H4 EQ0.*) admit.
+Admitted.
+
+(* Preservation of expression semantics with respect to small-step semantics *)
+(* Tweak lemma to not include cases where the expression take step to another expression *)
 Lemma sem_lexpr_preserve : forall m e m' e' ce,
 sem_expr bge benv m e m' e' ->
 is_lbeepl e = true ->
 transBeePL_expr_expr e = OK ce ->
-tr_expr_expr benv e ce ->
-exists ce', Csem.lred cge cenv ce m ce' m' /\ tr_expr_expr benv e' ce'.
+sim_bexpr_cexpr benv e ce ->
+exists ce', Csem.lred cge cenv ce m ce' m' /\ sim_bexpr_cexpr benv e' ce'.
 Proof.
-Admitted. 
+move=> m e m' e' ce he hl ht hs. elim: e he hl ht hs=> //=.
+(* Var *)
++ move=> v he _ ht htr. inversion he; subst. monadInv ht.
+  inversion htr; subst. 
+  (* local var *)
+  + exists (Csyntax.Eloc l Ptrofs.zero Full x). 
+    move: (H4 cenv (vname v)). case: ifP=> //= hs h.
+    + split=> //=.
+      + apply Csem.red_var_local. by move: (h l)=> [].
+      by apply sim_val_loc.
+    case: h=> //= h1 h2. by rewrite H0 in h1.
+  (* global var *)
+  monadInv ht. exists (Csyntax.Eloc l Ptrofs.zero Full x). split=> //=.
+  + apply Csem.red_var_global. inversion htr; subst.
+    move: (H5 cenv (vname v)). case: ifP=> //= h h'.
+    + rewrite /isSome in h. by rewrite H0 /= in h.
+    by case: h'=> //=.
+  + by rewrite symbols_preserved.
+  by apply sim_val_loc.
+(* Builtin: Deref *)
++ move=> [] //= es t he _ ht htr.
+  monadInv ht; subst. inversion he; subst; rewrite /=.
+  + rewrite /transBeePL_expr_exprs /= in EQ. monadInv EQ; subst.
+    rewrite /exprlist_list_expr /=. inversion htr; subst.  
+    admit.
+  rewrite /transBeePL_expr_exprs /= in EQ. monadInv EQ; subst.
+  rewrite /exprlist_list_expr /=. inversion htr; subst. 
+  exists (Eloc l ofs Full x0). split=> //=.
+  + monadInv EQ0; subst. rewrite H2 /=. apply Csem.red_deref.
+  by apply sim_addr.
+Admitted.
 
 Definition is_rbeepl (e : BeePL.expr) : bool :=
 match e with 
@@ -397,7 +734,7 @@ match e with
 | App id e es t => false  
 | Prim b es t => match b with 
                  | Ref => true
-                 | Deref => false 
+                 | Deref => true 
                  | Massgn => false 
                  | Uop o => true
                  | Bop o => true
@@ -414,8 +751,8 @@ Lemma sem_rexpr_preserve : forall m e m' e' ce,
 sem_expr bge benv m e m' e' ->
 is_rbeepl e = true ->
 transBeePL_expr_expr e = OK ce ->
-tr_expr_expr benv e ce ->
-exists ce' tr, Csem.rred cge ce m tr ce' m' /\ tr_expr_expr benv e' ce'.
+sim_bexpr_cexpr benv e ce ->
+exists ce' tr, Csem.rred cge ce m tr ce' m' /\ sim_bexpr_cexpr benv e' ce'.
 Proof.
 Admitted. 
 
